NLustre/SemEquiv.v
@@ -2,6 +2,7 @@ Require Import List.
 Import List.ListNotations.
 Open Scope list_scope.
 Require Import Coq.Sorting.Permutation.
+Require Import Morphisms.
 
 Require Import Coq.FSets.FMapPositive.
 Require Import Velus.Common.
@@ -111,7 +112,7 @@ Module Type SEMEQUIV
 
   Add Parametric Morphism
       A B (P: A -> Stream B -> Prop) xs
-      (P_compat: forall (x: A) (y y': Stream B), y ≡ y' -> (P x y <-> P x y'))
+      (P_compat: Proper (eq ==> @EqSt B ==> Basics.impl) P)
     : (@Forall2 A (Stream B) P xs)
       with signature @EqSts B ==> Basics.impl
         as Forall2_EqSt.
@@ -119,18 +120,28 @@ Module Type SEMEQUIV
     intros ys ys' Eys.
     revert xs ys ys' Eys;
       induction xs, ys; intros ** H; inv H; inv Eys; auto.
-    constructor; eauto.  eapply P_compat; eauto.
-    - now symmetry.
+    constructor; eauto.
+    - eapply P_compat; eauto.
     - eapply IHxs; eauto.
   Qed.
 
-  Add Parametric Morphism H x : (sem_var H x)
-      with signature @EqSt value ==> Basics.impl
+  Remark MapsTo_sem_var:
+    forall H x xs,
+      PM.MapsTo x xs H ->
+      sem_var H x xs.
+  Proof.
+    econstructor; eauto; reflexivity.
+  Qed.
+
+  Add Parametric Morphism H : (sem_var H)
+      with signature eq ==> @EqSt value ==> Basics.impl
         as sem_var_EqSt.
   Proof.
-    intros xs xs' E.
-    intros Sem.
-  Admitted.
+    intros x xs xs' E.
+    intros Sem; induction Sem.
+    econstructor; eauto.
+    transitivity xs; auto; symmetry; auto.
+  Qed.
 
   Add Parametric Morphism : merge
       with signature @EqSt value ==> @EqSt value ==> @EqSt value ==> @EqSt value ==> Basics.impl
@@ -341,12 +352,8 @@ Module Type SEMEQUIV
     - induction Sem.
       econstructor; eauto.
       + instantiate (1:=H).
-        eapply Forall2_EqSt; eauto.
-        intros; split; apply sem_var_EqSt; auto.
-        now symmetry.
-      + eapply Forall2_EqSt; eauto.
-        intros; split; apply sem_var_EqSt; auto.
-        now symmetry.
+        now rewrite <-Exss.
+      + now rewrite <-Eyss.
       + apply Forall_impl with (P:=Wire.sem_equation G H (clocks_of xss) r); auto.
         apply wire_sem_equation_morph_fix; auto.
         now rewrite Exss.
@@ -364,6 +371,26 @@ Module Type SEMEQUIV
         as wire_sem_node_morph.
   Proof.
     unfold Basics.impl; apply wire_sem_node_morph_fix.
+  Qed.
+
+  Add Parametric Morphism c : (const c)
+      with signature @EqSt bool ==> @EqSt value
+        as const_EqSt.
+  Proof.
+    cofix; intros b b' Eb.
+    unfold_Stv b; unfold_Stv b';
+      constructor; inv Eb; simpl in *; try discriminate; auto.
+  Qed.
+
+  Add Parametric Morphism A opaque n : (Rec.mask opaque n)
+      with signature @EqSt bool ==> @EqSt A ==> @EqSt A
+        as mask_EqSt.
+  Proof.
+    revert n; cofix Cofix; intros n rs rs' Ers xs xs' Exs.
+    unfold_Stv rs; unfold_Stv rs'; unfold_St xs; unfold_St xs';
+      constructor; inv Ers; inv Exs;
+        simpl in *; try discriminate;
+          destruct n as [|[]]; auto; try reflexivity.
   Qed.
 
   CoFixpoint false_s : Stream bool := false ::: false_s.
@@ -458,24 +485,223 @@ Module Type SEMEQUIV
         admit.
     Admitted.
 
-    Definition map_history: (Stream value -> Stream value) -> history -> history.
-    Admitted.
+    Definition map_history (f: Stream value -> Stream value) (H: history) : history :=
+      PM.map f H.
 
     Fact map_history_spec:
       forall H x xs f,
+        Proper (@EqSt value ==> @EqSt value) f ->
         sem_var H x xs ->
         sem_var (map_history f H) x (f xs).
-    Admitted.
+    Proof.
+      induction 2 as [? ? xs xs' Sem Exs].
+      econstructor.
+      - apply PM.map_1; eauto.
+      - rewrite Exs; reflexivity.
+    Qed.
 
     Definition mask_history (n: nat) (rs: Stream bool) (H: history) : history :=
-      map_history (Rec.mask n rs) H.
+      map_history (Rec.mask_v n rs) H.
 
     Corollary mask_history_spec:
       forall n rs H x xs,
         sem_var H x xs ->
-        sem_var (mask_history n rs H) x (Rec.mask n rs xs).
+        sem_var (mask_history n rs H) x (Rec.mask_v n rs xs).
     Proof.
       intros; apply map_history_spec; auto.
+      solve_proper.
+    Qed.
+
+    Corollary mask_history_spec_Forall2:
+      forall n rs H xs xss,
+        Forall2 (sem_var H) xs xss ->
+        Forall2 (sem_var (mask_history n rs H)) xs (List.map (Rec.mask_v n rs) xss).
+    Proof.
+      intros.
+      rewrite Forall2_map_2.
+      eapply Forall2_impl_In; eauto.
+      intros; apply mask_history_spec; auto.
+    Qed.
+
+        Remark const_false_absent:
+      forall c,
+        const c false_s ≡ Streams.const absent.
+    Proof.
+      cofix; constructor; simpl; auto.
+    Qed.
+
+    (* Remark mask_absent: *)
+    (*   forall n rs, *)
+    (*     Rec.mask n rs (Streams.const absent) ≡ Streams.const absent. *)
+    (* Proof. *)
+    (*   cofix; intros. *)
+    (*   unfold_Stv rs; constructor; destruct n as [|[]]; *)
+    (*     simpl; auto; reflexivity. *)
+    (* Qed. *)
+
+
+
+
+    (* Remark clocks_of_nil: *)
+    (*   clocks_of [] ≡ false_s. *)
+    (* Proof. *)
+    (*   cofix; constructor; simpl; auto. *)
+    (* Qed. *)
+
+    Remark mask_sem_const:
+      forall n rs c b,
+        Rec.mask_v n rs (const c b) ≡ const c (Rec.mask_b n rs b).
+    Proof.
+      cofix; intros.
+      unfold_Stv rs; unfold_Stv b; destruct n as [|[]];
+        constructor; simpl; auto;
+          rewrite const_false_absent; reflexivity.
+    Qed.
+
+    Remark when_absent:
+      forall k, when k (Streams.const absent) (Streams.const absent) (Streams.const absent).
+    Proof.
+      cofix;
+        rewrite (unfold_Stream (Streams.const absent));
+        simpl; constructor; auto.
+    Qed.
+
+    Corollary when_mask:
+      forall n rs k es xs os,
+        when k es xs os ->
+        when k (Rec.mask_v n rs es) (Rec.mask_v n rs xs) (Rec.mask_v n rs os).
+    Proof.
+      cofix; intros.
+      rewrite (unfold_Stream (Rec.mask_v n rs es));
+        rewrite (unfold_Stream (Rec.mask_v n rs xs));
+        rewrite (unfold_Stream (Rec.mask_v n rs os)).
+      unfold_Stv rs; unfold_Stv es; unfold_St xs; unfold_St os;
+        destruct n as [|[]]; try (now inv H; constructor; auto).
+      rewrite <-unfold_Stream; apply when_absent.
+      rewrite <-unfold_Stream; apply when_absent.
+    Qed.
+
+    Remark lift1_absent:
+      forall op t, lift1 op t (Streams.const absent) (Streams.const absent).
+    Proof.
+      cofix;
+        rewrite (unfold_Stream (Streams.const absent));
+        simpl; constructor; auto.
+    Qed.
+
+    Corollary lift1_mask:
+      forall n rs op t es os,
+        lift1 op t es os ->
+        lift1 op t (Rec.mask_v n rs es) (Rec.mask_v n rs os).
+    Proof.
+      cofix; intros.
+      rewrite (unfold_Stream (Rec.mask_v n rs es));
+        rewrite (unfold_Stream (Rec.mask_v n rs os)).
+      unfold_Stv rs; unfold_Stv es; unfold_St os;
+        destruct n as [|[]]; try (now inv H; constructor; auto).
+      rewrite <-unfold_Stream; apply lift1_absent.
+      rewrite <-unfold_Stream; apply lift1_absent.
+    Qed.
+
+    Remark lift2_absent:
+      forall op t1 t2, lift2 op t1 t2 (Streams.const absent) (Streams.const absent) (Streams.const absent).
+    Proof.
+      cofix;
+        rewrite (unfold_Stream (Streams.const absent));
+        simpl; constructor; auto.
+    Qed.
+
+    Corollary lift2_mask:
+      forall n rs op t1 t2 e1s e2s os,
+        lift2 op t1 t2 e1s e2s os ->
+        lift2 op t1 t2 (Rec.mask_v n rs e1s) (Rec.mask_v n rs e2s) (Rec.mask_v n rs os).
+    Proof.
+      cofix; intros.
+      rewrite (unfold_Stream (Rec.mask_v n rs e1s));
+        rewrite (unfold_Stream (Rec.mask_v n rs e2s));
+        rewrite (unfold_Stream (Rec.mask_v n rs os)).
+      unfold_Stv rs; unfold_Stv e1s; unfold_Stv e2s; unfold_St os;
+        destruct n as [|[]]; try (now inv H; constructor; auto).
+      rewrite <-unfold_Stream; apply lift2_absent.
+      rewrite <-unfold_Stream; apply lift2_absent.
+    Qed.
+
+    Lemma mask_sem_lexp:
+      forall n rs H b e es,
+        sem_lexp H b e es ->
+        sem_lexp (mask_history n rs H) (Rec.mask_b n rs b) e (Rec.mask_v n rs es).
+    Proof.
+      intros ** Sem; induction Sem.
+      - rewrite mask_sem_const; constructor.
+      - constructor; apply mask_history_spec; auto.
+      - econstructor; eauto.
+        + apply mask_history_spec; eauto.
+        + now apply when_mask.
+      - econstructor; eauto.
+        now apply lift1_mask.
+      - econstructor; eauto.
+        now apply lift2_mask.
+    Qed.
+
+     Remark merge_absent:
+      merge (Streams.const absent) (Streams.const absent) (Streams.const absent) (Streams.const absent).
+    Proof.
+      cofix;
+        rewrite (unfold_Stream (Streams.const absent));
+        simpl; constructor; auto.
+    Qed.
+
+    Corollary merge_mask:
+      forall n rs xs ts fs os,
+        merge xs ts fs os ->
+        merge (Rec.mask_v n rs xs) (Rec.mask_v n rs ts) (Rec.mask_v n rs fs) (Rec.mask_v n rs os).
+    Proof.
+      cofix; intros.
+      rewrite (unfold_Stream (Rec.mask_v n rs xs));
+        rewrite (unfold_Stream (Rec.mask_v n rs ts));
+        rewrite (unfold_Stream (Rec.mask_v n rs fs));
+        rewrite (unfold_Stream (Rec.mask_v n rs os)).
+      unfold_Stv rs; unfold_St xs; unfold_St ts; unfold_St fs; unfold_St os;
+        destruct n as [|[]]; try (now inv H; constructor; auto).
+      rewrite <-unfold_Stream; apply merge_absent.
+    Qed.
+
+    Remark ite_absent:
+      ite (Streams.const absent) (Streams.const absent) (Streams.const absent) (Streams.const absent).
+    Proof.
+      cofix;
+        rewrite (unfold_Stream (Streams.const absent));
+        simpl; constructor; auto.
+    Qed.
+
+    Corollary ite_mask:
+      forall n rs es ts fs os,
+        ite es ts fs os ->
+        ite (Rec.mask_v n rs es) (Rec.mask_v n rs ts) (Rec.mask_v n rs fs) (Rec.mask_v n rs os).
+    Proof.
+      cofix; intros.
+      rewrite (unfold_Stream (Rec.mask_v n rs es));
+        rewrite (unfold_Stream (Rec.mask_v n rs ts));
+        rewrite (unfold_Stream (Rec.mask_v n rs fs));
+        rewrite (unfold_Stream (Rec.mask_v n rs os)).
+      unfold_Stv rs; unfold_St es; unfold_St ts; unfold_St fs; unfold_St os;
+        destruct n as [|[]]; try (now inv H; constructor; auto).
+      rewrite <-unfold_Stream; apply ite_absent.
+    Qed.
+
+    Lemma mask_sem_cexp:
+      forall n rs H b e es,
+        sem_cexp H b e es ->
+        sem_cexp (mask_history n rs H) (Rec.mask_b n rs b) e (Rec.mask_v n rs es).
+    Proof.
+      intros ** Sem; induction Sem.
+      - econstructor; eauto.
+        + apply mask_history_spec; eauto.
+        + now apply merge_mask.
+      - econstructor; eauto.
+        + apply mask_sem_lexp; eauto.
+        + now apply ite_mask.
+      - constructor; apply mask_sem_lexp; auto.
     Qed.
 
     Lemma WireRec_node_reset:
@@ -491,16 +717,17 @@ Module Type SEMEQUIV
       intro i.
       econstructor; eauto.
       instantiate (1:=mask_history i (reset_of rs) H).
-      - admit.
-      - admit.
+      - now apply mask_history_spec_Forall2.
+      - now apply mask_history_spec_Forall2.
       - induction (n_eqs n) as [|e]; auto.
         inversion_clear Sem as [|? ? Sem_e].
         constructor; auto.
         remember (clocks_of ess) as b.
         remember (reset_of rs) as r.
-        induction Sem_e.
-        + apply (mask_history_spec i r)in H3.
+        induction Sem_e as [? ? ? ? ? ? ? Sem Sem_var| | |].
+        + apply (mask_history_spec i r) in Sem_var.
           econstructor; eauto.
+
       - econstructor; eauto.
       - econstructor. clear; induction xss.
         + eexists; eauto.
